CurryHowardCorrespondence.lean
@@ -10,4 +10,74 @@ theorem EQRemainsAfterTranslationTheory: ∀ {Γ Γ': Theory}, Γ = Γ' → theo
 
 
 
--- theorem soundness : ∀ {p : Formula} {Γ: Theory}, (h : Provable Γ p) → ∃ (A: Term) (Γ': Context) (t: Types), Inhabitable (theoryToContext Γ) (translateFormulaToType t) A
+theorem completeness : ∀ {p : Formula} {Γ: Theory}, (h : Provable Γ p) → ∃ (A: Term) , Inhabitable (theoryToContext Γ) (translateFormulaToType p) A
+| p, Γ, Provable.Axiom h => by
+  let Γ' := theoryToContext Γ
+  let t := translateFormulaToType p
+  let p' := translateFormulaToVarname p
+  let h' : Γ'.getType p' == t:= by
+    let h1 := t2c_cons h
+    simp [Γ']
+    exact h1
+  let A := Term.Var p'
+  let inh := Inhabitable.Var h'
+  simp [Γ'] at inh
+  exact ⟨A, inh⟩
+| Formula.And p q, Γ, Provable.AndIntro h1 h2  => by
+  let ⟨A1, inh1⟩ := completeness h1
+  let ⟨A2, inh2⟩ := completeness h2
+  let A := Term.Pair A1 A2
+  let inh := Inhabitable.Pair inh1 inh2
+  simp [translateFormulaToType]
+  exact ⟨A, inh⟩
+| Formula.Or p q, Γ, Provable.OrIntro1 h1 => by
+  let ⟨A1, inh1⟩ := completeness h1
+  let A:= Term.Inl A1 (translateFormulaToType p) (translateFormulaToType q)
+  let inh :Inhabitable (theoryToContext Γ) (Types.Either (translateFormulaToType p) (translateFormulaToType q)) A := Inhabitable.Inl inh1
+  simp [translateFormulaToType]
+  exact ⟨A, inh⟩
+| Formula.Or p q, Γ, Provable.OrIntro2 h1 => by
+  let ⟨A1, inh1⟩ := completeness h1
+  let A:= Term.Inr A1 (translateFormulaToType p) (translateFormulaToType q)
+  let inh :Inhabitable (theoryToContext Γ) (Types.Either (translateFormulaToType p) (translateFormulaToType q)) A := Inhabitable.Inr inh1
+  simp [translateFormulaToType]
+  exact ⟨A, inh⟩
+| Formula.Impl p q, Γ, Provable.ImpIntro h1 => by
+  let ⟨A1, inh1⟩ := completeness h1
+  simp [theoryToContext] at inh1
+  let inh := Inhabitable.Abs inh1
+  let A := Term.Abs (translateFormulaToVarname p) (translateFormulaToType p) A1
+  exact ⟨A, inh⟩
+| p, Γ, Provable.false_elim h => by
+  let ⟨A1, inh1⟩ := completeness h
+  simp [translateFormulaToType] at inh1
+  let A := Term.Absurd (translateFormulaToType p) A1
+  let inh :Inhabitable (theoryToContext Γ) (translateFormulaToType p) A := Inhabitable.Absurd inh1
+  exact ⟨A, inh⟩
+| p, Γ, Provable.ImpElim h1 h2 => by
+  let ⟨A1, inh1⟩ := completeness h1
+  let ⟨A2, inh2⟩ := completeness h2
+  simp [translateFormulaToType] at inh1
+  let inh := Inhabitable.App inh1 inh2
+  let A := Term.App A1 A2
+  exact ⟨A, inh⟩
+| p, Γ, Provable.OrElim h1 h2 h3 => by
+  let ⟨A1, inh1⟩ := completeness h1
+  let ⟨A2, inh2⟩ := completeness h2
+  let ⟨A3, inh3⟩ := completeness h3
+  simp [translateFormulaToType] at inh1
+  simp [theoryToContext] at inh2
+  simp [theoryToContext] at inh3
+  let inh := Inhabitable.Case inh1 inh2 inh3
+  let A := getInhabitableTerm inh
+  exact ⟨A, inh⟩
+| p , Γ, Provable.AndElim1 h1 => by
+  let ⟨A1, inh1⟩ := completeness h1
+  let A := Term.Proj1 A1
+  let inh := Inhabitable.Proj1 inh1
+  exact ⟨A, inh⟩
+| p, Γ, Provable.AndElim2 h1 => by
+  let ⟨A1, inh1⟩ := completeness h1
+  let A := Term.Proj2 A1
+  let inh := Inhabitable.Proj2 inh1
+  exact ⟨A, inh⟩
